lib/isabelle/State_monad_extras.thy
@@ -2,24 +2,42 @@ theory State_monad_extras
   imports State_monad
 begin
 
-lemma bind_ext_cong[fundef_cong]:
+abbreviation "bindS_aux f \<equiv> (\<lambda>r. case r of (Value a, s') \<Rightarrow> f a s' | (Ex e, s') \<Rightarrow> [(Ex e, s')])"
+
+lemma bindS_ext_cong[fundef_cong]:
   assumes m: "m1 s = m2 s"
     and f: "\<And>a s'. (Value a, s') \<in> set (m2 s) \<Longrightarrow> f1 a s' = f2 a s'"
-  shows "(bind m1 f1) s = (bind m2 f2) s"
+  shows "(bindS m1 f1) s = (bindS m2 f2) s"
 proof -
-  have "List.concat (map (\<lambda>x. case x of (Value a, s') \<Rightarrow> f1 a s' | (Exception e, s') \<Rightarrow> [(Exception e, s')]) (m2 s)) =
-        List.concat (map (\<lambda>x. case x of (Value a, s') \<Rightarrow> f2 a s' | (Exception e, s') \<Rightarrow> [(Exception e, s')]) (m2 s))"
+  have "List.concat (map (bindS_aux f1) (m2 s)) = List.concat (map (bindS_aux f2) (m2 s))"
     using f by (intro arg_cong[where f = List.concat]) (auto intro: map_ext split: result.splits)
-  then show ?thesis using m by (auto simp: bind_def)
+  then show ?thesis using m by (auto simp: bindS_def)
 qed
 
-lemma bind_cong[fundef_cong]:
+lemma bindS_cong[fundef_cong]:
   assumes m: "m1 = m2"
     and f: "\<And>s a s'. (Value a, s') \<in> set (m2 s) \<Longrightarrow> f1 a s' = f2 a s'"
-  shows "bind m1 f1 = bind m2 f2"
-  using assms by (blast intro: bind_ext_cong)
+  shows "bindS m1 f1 = bindS m2 f2"
+  using assms by (blast intro: bindS_ext_cong)
 
-lemma bind_return[simp]: "bind (return x) m = m x"
-  by (auto simp add: bind_def return_def)
+lemma bindS_returnS[simp]: "bindS (returnS x) m = m x"
+  by (auto simp add: bindS_def returnS_def)
+
+lemma bindS_assoc[simp]: "bindS (bindS m f) g = bindS m (\<lambda>x. bindS (f x) g)"
+proof -
+  have "List.concat (map (bindS_aux g) (List.concat (map (bindS_aux f) xs))) =
+        List.concat (map (bindS_aux (\<lambda>x s. List.concat (map (bindS_aux g) (f x s)))) xs)" for xs
+    by (induction xs) (auto split: result.splits)
+  then show ?thesis unfolding bindS_def by auto
+qed
+
+lemma bindS_failS[simp]: "bindS (failS msg) f = failS msg" by (auto simp: bindS_def failS_def)
+lemma bindS_throwS[simp]: "bindS (throwS e) f = throwS e" by (auto simp: bindS_def throwS_def)
+declare seqS_def[simp]
+
+lemma try_catchS_returnS[simp]: "try_catchS (returnS a) h = returnS a"
+  and try_catchS_failS[simp]: "try_catchS (failS msg) h = failS msg"
+  and try_catchS_throwS[simp]: "try_catchS (throwS e) h = h e"
+  by (auto simp: returnS_def failS_def throwS_def try_catchS_def)
 
 end
