lib/isabelle/State_extras.thy
@@ -1,0 +1,35 @@
+theory State_extras
+  imports State
+begin
+
+lemma All_liftState_dom: "liftState_dom (r, m)"
+  by (induction m) (auto intro: liftState.domintros)
+
+termination liftState using All_liftState_dom by auto
+
+lemma liftState_return[simp]: "liftState r (return a) = returnS a" by (auto simp: return_def)
+lemma liftState_throw[simp]: "liftState r (throw e) = throwS e" by (auto simp: throw_def)
+lemma liftState_assert[simp]: "liftState r (assert_exp c msg) = assert_expS c msg" by (auto simp: assert_exp_def assert_expS_def)
+
+lemma liftState_bind[simp]:
+  "liftState r (bind m f) = bindS (liftState r m) (liftState r \<circ> f)"
+  by (induction m f rule: bind.induct) auto
+
+lemma liftState_read_reg[intro]:
+  assumes "\<And>s. Option.bind (get_regval' (name reg) s) (of_regval reg) = Some (read_from reg s)"
+  shows "liftState (get_regval', set_regval') (read_reg reg) = read_regS reg"
+proof
+  fix s :: "'a sequential_state"
+  obtain rv v where "get_regval' (name reg) (regstate s) = Some rv"
+    and "of_regval reg rv = Some v" and "read_from reg (regstate s) = v"
+    using assms unfolding bind_eq_Some_conv by blast
+  then show "liftState (get_regval', set_regval') (read_reg reg) s = read_regS reg s"
+    by (auto simp: read_reg_def bindS_def returnS_def read_regS_def)
+qed
+
+lemma liftState_write_reg[intro]:
+  assumes "\<And>s. set_regval' (name reg) (regval_of reg v) s = Some (write_to reg s v)"
+  shows "liftState (get_regval', set_regval') (write_reg reg v) = write_regS reg v"
+  using assms by (auto simp: write_reg_def bindS_def returnS_def write_regS_def)
+
+end
