riscv/Makefile
@@ -3,7 +3,7 @@ SAIL_DIR ?= $(realpath ..)
 
 export SAIL_DIR
 
-all: riscv Riscv_embed_sequential.thy
+all: riscv Riscv.thy
 
 check: $(SAIL_SRCS) main.sail
 	$(SAIL_DIR)/sail $^
@@ -14,28 +14,28 @@ riscv: $(SAIL_SRCS) main.sail
 riscv_duopod_ocaml: prelude.sail riscv_duopod.sail
 	$(SAIL_DIR)/sail -ocaml -o $@ $^
 
-riscv_duopod_embed_sequential.lem: prelude.sail riscv_duopod.sail
-	$(SAIL_DIR)/sail -lem -lem_sequential -lem_mwords -lem_lib Riscv_extras_embed -o riscv_duopod $^
-Riscv_duopod_embed_sequential.thy: riscv_duopod_embed_sequential.lem riscv_extras_embed_sequential.lem
+riscv_duopod.lem: prelude.sail riscv_duopod.sail
+	$(SAIL_DIR)/sail -lem -lem_mwords -lem_lib Riscv_extras -o riscv_duopod $^
+Riscv_duopod.thy: riscv_duopod.lem riscv_extras.lem
 	lem -isa -outdir . -lib ../src/lem_interp -lib ../src/gen_lib \
-		riscv_extras_embed_sequential.lem \
-		riscv_duopod_embed_types_sequential.lem \
-		riscv_duopod_embed_sequential.lem
+		riscv_extras.lem \
+		riscv_duopod_types.lem \
+		riscv_duopod.lem
 
-riscv_duopod: riscv_duopod_ocaml Riscv_duopod_embed_sequential.thy
+riscv_duopod: riscv_duopod_ocaml Riscv_duopod.thy
 
-Riscv_embed_sequential.thy: riscv_embed_sequential.lem riscv_extras_embed_sequential.lem
+Riscv.thy: riscv.lem riscv_extras.lem
 	lem -isa -outdir . -lib ../src/lem_interp -lib ../src/gen_lib \
-		riscv_extras_embed_sequential.lem \
-		riscv_embed_types_sequential.lem \
-		riscv_embed_sequential.lem
+		riscv_extras.lem \
+		riscv_types.lem \
+		riscv.lem
 
-riscv_embed_sequential.lem: $(SAIL_SRCS)
-	$(SAIL_DIR)/sail -lem -o riscv -lem_sequential -lem_mwords -lem_lib Riscv_extras_embed $^
+riscv.lem: $(SAIL_SRCS)
+	$(SAIL_DIR)/sail -lem -o riscv -lem_mwords -lem_lib Riscv_extras $^
 
 clean:
 	-rm -rf riscv _sbuild
-	-rm -f riscv_embed_sequential.lem riscv_embed_types_sequential.lem
-	-rm -f Riscv_embed_sequential.thy Riscv_embed_types_sequential.thy \
-		Riscv_extras_embed_sequential.thy
-	-rm -f Riscv_duopod_embed_sequential.thy Riscv_duopod_embed_types_sequential.thy riscv_duopod_embed_sequential.lem riscv_duopod_embed_types_sequential.lem
+	-rm -f riscv.lem riscv_types.lem
+	-rm -f Riscv.thy Riscv_types.thy \
+		Riscv_extras.thy
+	-rm -f Riscv_duopod.thy Riscv_duopod_types.thy riscv_duopod.lem riscv_duopod_types.lem
